src/examples/parallel_add.v
@@ -1,4 +1,4 @@
-From iris_simp_lang Require Import simp examples.par.
+From iris_simp_lang Require Import simp adequacy examples.par.
 From iris.bi.lib Require Import fractional.
 From iris.base_logic.lib Require Import ghost_var.
 From iris Require Import options.
@@ -13,18 +13,18 @@ Definition parallel_add: expr :=
 Section proof.
   Context `{!simpG Σ, !spawnG Σ, !ghost_varG Σ Z}.
 
-  Definition parallel_add_inv_2 (r : loc) (γ1 γ2 : gname) : iProp Σ :=
+  Definition parallel_add_inv (r : loc) (γ1 γ2 : gname) : iProp Σ :=
     ∃ n1 n2 : Z, r ↦ #(n1 + n2) ∗
                  ghost_var γ1 (1/2) n1 ∗ ghost_var γ2 (1/2) n2.
 
-  Lemma parallel_add_spec_2 :
+  Lemma parallel_add_spec :
     {{{ True }}} parallel_add {{{ RET #4; True }}}.
   Proof using All.
     iIntros (Φ) "_ Post".
     unfold parallel_add. wp_alloc r as "Hr". wp_let.
     iMod (ghost_var_alloc 0) as (γ1) "[Hγ1 Hγ1●]".
     iMod (ghost_var_alloc 0) as (γ2) "[Hγ2 Hγ2●]".
-    iMod (inv_alloc nroot _ (parallel_add_inv_2 r γ1 γ2) with "[Hr Hγ1● Hγ2●]") as "#Hinv".
+    iMod (inv_alloc nroot _ (parallel_add_inv r γ1 γ2) with "[Hr Hγ1● Hγ2●]") as "#Hinv".
     { iExists 0, 0. iFrame. }
     wp_apply (wp_par (λ _, ghost_var γ1 (1/2) 2) (λ _, ghost_var γ2 (1/2) 2)
                 with "[Hγ1] [Hγ2]").
@@ -54,3 +54,34 @@ Section proof.
   Qed.
 
 End proof.
+
+(*|
+===============
+Using adequacy
+===============
+
+We proved an Iris specification, but what does it really mean about the program? We can use the simp_lang adequacy theorem to "extract" the pure post-postcondition into a statement about the execution semantics.
+
+The Iris triple says two things, which are bundled into the `adequate` definition used by `simp_adequacy`: `parallel_add` will not get stuck, and if it terminates in a value, that value will be 4. We'll only make use of the second part here.
+
+To use adequacy and this triple, we'll finally gather up all the functors needed for Iris ghost state and produce one of the Σ assumptions used in all of our proofs; it has all the ghost state needed for the features used in this proof.
+
+Note that we aren't in a section and this theorem statement only refers to the language semantics, so we've eliminated Iris from our trusted computing base! The theorem refers to the semantics through erased_step, which ignores observations; this doesn't matter for this language because we aren't using prophecy variables.
+|*)
+
+Definition parallel_addΣ: gFunctors :=
+  #[simpΣ; spawnΣ; ghost_varΣ Z].
+
+Lemma parallel_add_returns_4 σ σ' v :
+  rtc erased_step ([parallel_add], σ) ([Val v], σ') →
+  v = LitV (LitInt 4).
+Proof.
+  intros Hstep.
+  cut (adequate NotStuck parallel_add σ (λ v _, v = LitV (LitInt 4))).
+  { intros H. eapply adequate_alt in H as [Hval _]; eauto. }
+  apply (simp_adequacy parallel_addΣ).
+  intros.
+  by iApply (parallel_add_spec with "[//]").
+Qed.
+
+Print Assumptions parallel_add_returns_4.
